zoo_saturn/ws_bdeque_2: Fix.

lib/zoo_saturn/ws_bdeque_2.ml
@@ -21,11 +21,15 @@ let steal t =
   | None ->
       None
   | Some slot ->
-      Some !slot
+      let v = !slot in
+      slot := Obj.magic () ;
+      Some v
 
 let pop t =
   match Ws_bdeque_1.pop t with
   | None ->
       None
   | Some slot ->
-      Some !slot
+      let v = !slot in
+      slot := Obj.magic () ;
+      Some v
