theories/zoo_saturn/ws_bdeque_2__code.v
@@ -32,7 +32,9 @@ Definition ws_bdeque_2_steal : val :=
     | None =>
         §None
     | Some "slot" =>
-        ‘Some( !"slot" )
+        let: "v" := !"slot" in
+        "slot" <- () ;;
+        ‘Some( "v" )
     end.
 
 Definition ws_bdeque_2_pop : val :=
@@ -41,5 +43,7 @@ Definition ws_bdeque_2_pop : val :=
     | None =>
         §None
     | Some "slot" =>
-        ‘Some( !"slot" )
+        let: "v" := !"slot" in
+        "slot" <- () ;;
+        ‘Some( "v" )
     end.
